examples/n_german/nMutual219.thy
@@ -1,0 +1,392 @@
+theory nMutual219
+  imports CMP
+begin
+
+
+subsection \<open>Definitions\<close>
+
+text \<open>Represents the four states: idle, try, critical, exit\<close>
+
+definition I :: scalrValueType where [simp]: "I \<equiv> enum ''control'' ''I''"
+definition T :: scalrValueType where [simp]: "T \<equiv> enum ''control'' ''T''"
+definition C :: scalrValueType where [simp]: "C \<equiv> enum ''control'' ''C''"
+definition E :: scalrValueType where [simp]: "E \<equiv> enum ''control'' ''E''"
+
+definition true :: scalrValueType where [simp]: "true \<equiv> boolV True"
+definition false :: scalrValueType where [simp]: "false \<equiv> boolV False"
+
+text \<open>Initial condition: all processes in idle.
+  \<forall>i. n[i] = I
+\<close>
+definition initSpec0 :: "nat \<Rightarrow> formula" where
+  "initSpec0 N \<equiv> (\<forall>\<^sub>fi. IVar (Para ''n'' i) =\<^sub>f Const I) N"
+
+text \<open>Initial condition: x is True
+  x = True
+\<close>
+definition initSpec1 :: formula where
+  "initSpec1 \<equiv> IVar (Ident ''x'') =\<^sub>f Const true"
+
+text \<open>There cannot be one state in exit and another in critical or exit.
+  n[i] = E \<longrightarrow> (\<forall>j. i \<noteq> j \<longrightarrow> n[j] \<noteq> C \<and> n[j] \<noteq> E)
+\<close>
+definition invAux :: "nat \<Rightarrow> nat \<Rightarrow> formula" where
+  "invAux N i \<equiv> IVar (Para ''n'' i) =\<^sub>f Const E \<longrightarrow>\<^sub>f forallFormExcl 
+    (\<lambda>j. \<not>\<^sub>f IVar (Para ''n'' j) =\<^sub>f Const C \<and>\<^sub>f \<not>\<^sub>f IVar (Para ''n'' j) =\<^sub>f Const E) i N"  
+
+text \<open>Try enter critical region
+  n[i] = I \<rightarrow> n[i] := T
+\<close>
+definition n_Try :: "nat \<Rightarrow> rule" where
+  "n_Try i \<equiv>
+    IVar (Para ''n'' i) =\<^sub>f Const I
+   \<triangleright>
+    assign (Para ''n'' i, Const T)"
+
+text \<open>Enter critical region
+  n[i] = T \<and> x = True \<rightarrow> n[i] := C; x := False
+\<close>
+definition n_Crit :: "nat \<Rightarrow> rule" where
+  "n_Crit i \<equiv>
+    IVar (Para ''n'' i) =\<^sub>f Const T \<and>\<^sub>f
+    IVar (Ident ''x'') =\<^sub>f Const true
+   \<triangleright>
+    assign (Para ''n'' i, Const C) ||
+    assign (Ident ''x'', Const false)"
+
+text \<open>Exit critical region
+  n[i] = C \<rightarrow> n[i] := E
+\<close>
+definition n_Exit :: "nat \<Rightarrow> rule" where
+  "n_Exit i \<equiv>
+    IVar (Para ''n'' i) =\<^sub>f Const C
+   \<triangleright>
+    assign (Para ''n'' i, Const E)"
+
+text \<open>Move to idle
+  n[i] = E \<rightarrow> n[i] := I; x := True
+\<close>
+definition n_Idle :: "nat \<Rightarrow> rule" where
+  "n_Idle i \<equiv>
+    IVar (Para ''n'' i) =\<^sub>f Const E
+   \<triangleright>
+    assign (Para ''n'' i, Const I) ||
+    assign (Ident ''x'', Const true)"
+
+subsection \<open>References\<close>
+
+definition n_Crit_abs :: rule where
+  "n_Crit_abs \<equiv>
+    IVar (Ident ''x'') =\<^sub>f Const (boolV True)
+   \<triangleright>
+    assign (Ident ''x'', Const (boolV False))"
+
+definition n_Idle_abs1 :: rule where
+  "n_Idle_abs1 \<equiv>
+    chaos \<triangleright> assign (Ident ''x'', Const true)"
+
+definition n_Idle_abs2 :: "nat \<Rightarrow> rule" where
+"n_Idle_abs2 M \<equiv>
+    (\<forall>\<^sub>fj. ((\<not>\<^sub>f IVar (Para ''n'' j) =\<^sub>f Const (enum ''control'' ''C''))\<and>\<^sub>f
+      (\<not>\<^sub>f IVar (Para ''n'' j) =\<^sub>f Const (enum ''control'' ''E'')))) M 
+   \<triangleright>
+    assign (Ident ''x'', Const (boolV True))"
+
+
+subsection \<open>Individual tests\<close>
+
+lemma absInitSpec:
+  assumes "M \<le> N"
+  shows "absTransfForm M (initSpec0 N) = initSpec0 M"
+        "absTransfForm M initSpec1 = initSpec1"
+  unfolding initSpec0_def initSpec1_def using assms by auto
+
+lemma symInvAux:
+  "symParamForm N (invAux N)"
+  unfolding invAux_def
+  apply (auto intro!: symParamFormImply symParamFormAnd symParamFormForall symParamFormForallExcl)
+  unfolding symParamForm_def symParamForm2_def equivForm_def by auto
+
+lemma symTry:
+  "symParamRule N n_Try"
+  "wellFormedRule N (n_Try i)"
+  "absTransfRule M (n_Try i) = (if i \<le> M then n_Try i else chaos \<triangleright> skip)"
+  unfolding n_Try_def symParamRule_def by auto
+
+lemma symCrit:
+  "symParamRule N n_Crit"
+  "wellFormedRule N (n_Crit i)"
+  "absTransfRule M (n_Crit i) = (if i \<le> M then n_Crit i else n_Crit_abs)"
+  unfolding n_Crit_def n_Crit_abs_def symParamRule_def by auto
+
+lemma symExit:
+  "symParamRule N n_Exit"
+  "wellFormedRule N (n_Exit i)"
+  "absTransfRule M (n_Exit i) = (if i \<le> M then n_Exit i else chaos \<triangleright> skip)"
+  unfolding n_Exit_def symParamRule_def by auto
+
+lemma symIdle:
+  "symParamRule N n_Idle"
+  "wellFormedRule N (n_Idle i)"
+  "absTransfRule M (n_Idle i) = (if i \<le> M then n_Idle i else n_Idle_abs1)"
+  unfolding n_Idle_def n_Idle_abs1_def symParamRule_def by auto
+
+text \<open>Move to idle, strengthened:
+  n[i] = E \<and>
+  (\<forall>j. i \<noteq> j \<longrightarrow> n[j] \<noteq> C) \<and>
+  (\<forall>j. i \<noteq> j \<longrightarrow> n[j] \<noteq> E) \<rightarrow> n[i] := I; x := True
+\<close>
+definition n_Idle2_ref :: "nat \<Rightarrow> nat \<Rightarrow> rule" where
+  "n_Idle2_ref N i \<equiv>
+    IVar (Para ''n'' i) =\<^sub>f Const E \<and>\<^sub>f
+    forallFormExcl (\<lambda>j.( \<not>\<^sub>f IVar (Para ''n'' j) =\<^sub>f Const C)  \<and>\<^sub>f
+       \<not>\<^sub>f IVar (Para ''n'' j) =\<^sub>f Const E) i N
+   \<triangleright>
+    assign (Para ''n'' i, Const I) ||
+    assign (Ident ''x'', Const true)"
+ 
+lemma n_Idle2Eq:
+  "strengthenRule2 (invAux N i) (n_Idle i) = n_Idle2_ref N i"
+  by (auto simp add: strengthenRule2.simps invAux_def n_Idle_def n_Idle2_ref_def)
+
+lemma wellFormedIdle2:
+  "symParamRule N (n_Idle2_ref N)"
+  "wellFormedRule N (n_Idle2_ref N i)"
+  unfolding n_Idle2_ref_def
+   apply (auto intro!: symParamRuleI symParamFormAnd symParamFormForallExcl)
+  unfolding symParamForm_def symParamForm2_def symParamStatement_def by auto
+
+lemma absIdle2:
+  "M \<le> N \<Longrightarrow> absTransfRule M (n_Idle2_ref N i) = (if i \<le> M then n_Idle i else n_Idle_abs2 M)"
+  unfolding n_Idle_def n_Idle_abs2_def n_Idle2_ref_def by auto
+
+
+subsection \<open>Putting everything together\<close>
+
+definition n_Trys :: "nat \<Rightarrow> rule set" where
+  "n_Trys N \<equiv> oneParamCons N n_Try"
+
+definition n_Crits :: "nat \<Rightarrow> rule set" where
+  "n_Crits N \<equiv> oneParamCons N n_Crit"
+
+definition n_Exits :: "nat \<Rightarrow> rule set" where
+  "n_Exits N \<equiv> oneParamCons N n_Exit"
+
+definition n_Idles :: "nat \<Rightarrow> rule set" where
+  "n_Idles N \<equiv> oneParamCons N n_Idle"
+
+definition rules' :: "nat \<Rightarrow> rule set" where
+  "rules' N \<equiv> n_Trys N \<union> n_Crits N \<union> n_Exits N \<union> n_Idles N"
+
+lemma n_TrysIsSym:
+  "symProtRules' N (n_Trys N)"
+  using symTry(1) n_Trys_def symParaRuleInfSymRuleSet by auto
+
+lemma n_CritsIsSym:
+  "symProtRules' N (n_Crits N)"
+  using n_Crits_def symCrit(1) symParaRuleInfSymRuleSet by auto 
+
+lemma n_ExitsIsSym:
+  "symProtRules' N (n_Exits N)"
+  using n_Exits_def symExit(1) symParaRuleInfSymRuleSet by auto 
+
+lemma n_IdlesIsSym:
+  "symProtRules' N (n_Idles N)"
+  using n_Idles_def symIdle(1) symParaRuleInfSymRuleSet by auto
+
+lemma rulesSym':
+  "symProtRules' N (rules' N)"
+  unfolding rules'_def apply (intro symProtRulesUnion)
+  using n_CritsIsSym n_ExitsIsSym n_IdlesIsSym n_TrysIsSym by auto
+ 
+definition pair1 :: "(nat \<Rightarrow> formula) \<times> (nat \<Rightarrow> formula)" where
+  "pair1 \<equiv> (\<lambda>i. IVar (Para ''n'' i) =\<^sub>f Const E,
+            \<lambda>j. \<not>\<^sub>f IVar (Para ''n'' j) =\<^sub>f Const C \<and>\<^sub>f \<not>\<^sub>f IVar (Para ''n'' j) =\<^sub>f Const E)"
+
+definition F :: "((nat \<Rightarrow> formula) \<times> (nat \<Rightarrow> formula)) set" where
+  "F \<equiv> {pair1}"
+
+
+definition n_Idle2s :: "nat \<Rightarrow> rule set" where
+  "n_Idle2s N \<equiv> oneParamCons N (\<lambda>i. strengthenRule2 (constrInvByExcl pair1 i N) (n_Idle i))"
+
+
+definition rules2' :: "nat \<Rightarrow> rule set" where
+  "rules2' N \<equiv> n_Trys N \<union> n_Crits N \<union> n_Exits N \<union> n_Idle2s N"
+
+lemma n_Idle2sIsSym:
+  "symProtRules' N (n_Idle2s N)"
+  unfolding n_Idle2s_def
+  apply (rule symParaRuleInfSymRuleSet)
+  using invAux_def n_Idle2Eq wellFormedIdle2(1) constrInvByExcl_def
+  by (auto simp add: pair1_def)
+ 
+lemma rule2'IsSym:
+  "symProtRules' N (rules2' N)"
+  unfolding rules2'_def
+  apply (intro symProtRulesUnion)
+  using n_CritsIsSym n_ExitsIsSym n_Idle2sIsSym n_TrysIsSym by auto 
+
+definition type_inv :: "nat \<Rightarrow> state \<Rightarrow> bool" where
+  "type_inv N s = (\<forall>i. i \<le> N \<longrightarrow> s (Para ''n'' i) = I \<or> s (Para ''n'' i) = T \<or> s (Para ''n'' i) = C \<or> s (Para ''n'' i) = E)"
+
+lemma n_Try_type [intro]:
+  "type_inv N sk \<Longrightarrow> i \<le> N \<Longrightarrow> type_inv N (trans1 (act (n_Try i)) sk)"
+  unfolding type_inv_def n_Try_def by auto
+
+lemma n_Crit_type [intro]:
+  "type_inv N sk \<Longrightarrow> i \<le> N \<Longrightarrow> type_inv N (trans1 (act (n_Crit i)) sk)"
+  unfolding type_inv_def n_Crit_def by auto
+
+lemma n_Exit_type [intro]:
+  "type_inv N sk \<Longrightarrow> i \<le> N \<Longrightarrow> type_inv N (trans1 (act (n_Exit i)) sk)"
+  unfolding type_inv_def n_Exit_def by auto
+
+lemma n_Idle2s_type [intro]:
+  "type_inv N sk \<Longrightarrow> i \<le> N \<Longrightarrow> 
+type_inv N (trans1 (act (strengthenRule2 (constrInvByExcl pair1 i N) (n_Idle i))) sk)"
+  unfolding type_inv_def strengthenRule2.simps n_Idle_def by auto
+
+lemma invOnStateOfN' [simp,intro]:
+  assumes "reachableUpTo ({initSpec0 N} \<union> {initSpec1}) (rules2' N) k s"
+  shows "type_inv N s"
+  apply (rule invIntro[OF _ _ assms])
+  subgoal for s
+    by (auto simp add: type_inv_def initSpec0_def)
+  subgoal for r sk
+    unfolding rules2'_def by (auto simp add: n_Trys_def n_Crits_def n_Exits_def n_Idle2s_def)
+  done
+
+lemma invOnStateOfN'' [simp,intro]:
+  assumes a: "reachableUpTo fs rs k s"
+  shows "fs = {initSpec0 N} \<union> {initSpec1} \<longrightarrow> rs = rules2' N \<longrightarrow> i \<le> N \<longrightarrow> isEnumVal s (Para ''n'' i)"
+  using invOnStateOfN' unfolding type_inv_def C_def E_def I_def T_def
+  by (metis assms getValueType.simps(1) isEnumVal_def typeOf_def)
+
+lemma symPreds:
+  "symPredSet' N ({initSpec0 N} \<union> {initSpec1})"
+  apply (rule symPredsUnion)
+  subgoal
+    unfolding initSpec0_def
+    apply (rule symPredSetForall)
+    unfolding symParamForm_def by auto    
+  subgoal
+    unfolding symPredSet'_def initSpec1_def by auto
+  done
+
+
+lemma absTrys:
+  "M < N \<Longrightarrow> absTransfRule M ` (n_Trys N) = (n_Trys M) \<union> {chaos \<triangleright> skip}"
+  unfolding n_Trys_def apply (rule absGen) using symTry(3) by auto
+
+lemma absExits:
+  "M < N \<Longrightarrow> absTransfRule M ` (n_Exits N) = (n_Exits M) \<union> {chaos \<triangleright> skip}"
+  unfolding n_Exits_def apply (rule absGen) using symExit(3) by auto
+
+lemma absCrits:
+  "M < N \<Longrightarrow> absTransfRule M ` (n_Crits N) = (n_Crits M) \<union> {n_Crit_abs}"
+  unfolding n_Crits_def apply (rule absGen) using symCrit(3) by auto
+
+lemma n_Idle2_ref':
+  "strengthenRule2 (constrInvByExcl pair1 i N) (n_Idle i) = n_Idle2_ref N i"
+  unfolding n_Idle2_ref_def n_Idle_def constrInvByExcl_def pair1_def fst_conv snd_conv
+  by (auto simp add: strengthenRule2.simps)
+thm strengthenRule2.simps
+lemma absIdle2s:
+  "M < N \<Longrightarrow> absTransfRule M ` (n_Idle2s N) = (n_Idles M) \<union> {n_Idle_abs2 M}"
+  unfolding n_Idle2s_def n_Idles_def n_Idle2_ref'
+  apply (rule absGen) using absIdle2 by auto
+
+definition absRules :: "nat \<Rightarrow> rule set" where
+  "absRules M \<equiv> n_Trys M \<union> n_Exits M \<union> n_Crits M \<union> n_Idles M \<union>
+    {chaos \<triangleright> skip, n_Crit_abs, n_Idle_abs2 M}"
+
+lemma absAll:
+  "M < N \<Longrightarrow> absTransfRule M ` rules2' N = absRules M"
+  unfolding rules2'_def absRules_def image_Un absTrys absExits absCrits absIdle2s by auto
+
+text \<open>Final result for nMutual
+  a4 to be checked using model checker
+\<close>
+lemma absProtSim:
+  assumes a2: "M < N"
+    and a3: "M = 1"
+    and a4: "\<forall>i f s.
+       f \<in> F \<longrightarrow>
+       reachableUpTo {f'. \<exists>f. f \<in> {initSpec0 N} \<union> {initSpec1} \<and> f' = absTransfForm M f}
+        (absRules M) i s \<longrightarrow>
+       formEval (constrInv f 0 1) s"
+  shows "\<forall>f s. f \<in> constrInvByExcls F N \<longrightarrow> 
+    reachableUpTo ({initSpec0 N} \<union> {initSpec1}) (rules' N) i s \<longrightarrow> formEval f s"
+proof (rule_tac ?rs2.0="rules2' N" in CMP)
+  show "\<And>r. r \<in> rules' N \<longrightarrow> wellFormedRule N r"
+    by (auto simp add: rules'_def n_Trys_def symTry(2) n_Crits_def symCrit(2)
+                       n_Exits_def symExit(2) n_Idles_def symIdle(2))
+next
+  show "\<forall>f. f \<in> F \<longrightarrow> symPair f N"
+    by (auto simp add: F_def pair1_def symParamForm_def)
+next
+  show "symProtRules' N (rules' N)"
+    using rulesSym' by blast
+next
+  show "symPredSet' N ({initSpec0 N} \<union> {initSpec1})"
+    using symPreds by blast
+next
+  show "M \<le> N"
+    using a2 by arith
+next
+  show "\<forall>s i f. reachableUpTo ({initSpec0 N} \<union> {initSpec1}) (rules2' N) i s \<longrightarrow>
+        f \<in> F \<longrightarrow> (\<forall>v. v \<in> varOfForm (constrInv f 0 1) \<longrightarrow> s v = abs1 M s v)"
+    using invOnStateOfN'' enumValAbsRemainSame
+    unfolding F_def pair1_def using a2 a3 by auto
+next
+  show "\<forall>r'. r' \<in> rules2' N \<longrightarrow>
+         (\<exists>r f i. f \<in> F \<and> r \<in> rules' N \<and> i \<le> N \<and> r' = strengthenRule2 (constrInvByExcl f i N) r) \<or>
+         r' \<in> rules' N"
+  proof -
+    have "\<exists>r f i. f \<in> F \<and> r \<in> rules' N \<and> i \<le> N \<and> r' = strengthenRule2 (constrInvByExcl f i N) r"
+      if "r' \<in> n_Idle2s N" for r'
+      using that apply (auto simp add: n_Idle2s_def)
+      subgoal for i
+        apply (rule exI[where x="n_Idle i"])
+        unfolding F_def pair1_def by (auto simp add: constrInvByExcl_def strengthenRule2.simps n_Idle_def rules'_def n_Idles_def)
+      done
+    then show ?thesis
+      apply (unfold rules2'_def rules'_def) by auto
+  qed
+next
+  show "symProtRules' N (rules2' N)"
+    using rule2'IsSym by blast 
+next
+  show "\<forall>r. r \<in> rules' N \<longrightarrow>
+    (\<exists>f. f \<in> constrInvByExcls F N \<and> strengthenRule2 f r \<in> rules2' N) \<or> r \<in> rules2' N"
+  proof -
+    have "\<exists>f. f \<in> constrInvByExcls F N \<and> strengthenRule2 f r \<in> n_Trys N \<union> n_Crits N \<union> n_Exits N \<union> n_Idle2s N"
+      if "r \<in> n_Idles N" for r
+      using that apply (auto simp add: n_Idles_def)
+      subgoal for i
+        apply (rule exI[where x="constrInvByExcl pair1 i N"])
+        by (auto simp add: F_def pair1_def constrInvByExcl_def strengthenRule2.simps n_Idle2s_def)
+      done
+    then show ?thesis
+      apply (unfold rules2'_def rules'_def) by auto
+  qed
+next 
+  show "1 \<le> N"
+    using a2 a3 by arith  
+next 
+  show "\<forall>i f s.
+       f \<in> F \<longrightarrow>
+       reachableUpTo {f'. \<exists>f. f \<in> {initSpec0 N} \<union> {initSpec1} \<and> f' = absTransfForm M f}
+        {r'. \<exists>r. r \<in> rules2' N \<and> r' = absTransfRule M r} i s \<longrightarrow>
+       formEval (constrInv f 0 1) s"
+  proof -
+    have a: "{r'. \<exists>r. r \<in> rules2' N \<and> r' = absTransfRule M r} = absTransfRule M ` (rules2' N)"
+      by auto
+    show ?thesis
+      unfolding a absAll[OF a2]
+      using a2 a3 a4 absAll by auto
+  qed
+qed
+
+end
